\chapter*{Real Numbers}
\begin{definition}[Properties of real numbers] Properties of $\R$ are
    
    % (a).
    
    % (b).
    
    (d). $\exists$ an order on  $\R$ which means $\forall x,y \in \R, x < y \text{ or }, x > y, \text{ or } x = y$
    Ordering follows the following properties, 

    \qquad (1). $x < y, y < z \Rightarrow x < z$ (transitivity)
    
    \qquad (2). $x < y \Rightarrow x + z < y + z, \forall z \in \R$
    
    \qquad (3). $x < y, z > 0 \Rightarrow xz < yz$
\end{definition}

\begin{theorem}
    $xy = 0 \iff x = 0 \text{ or } y = 0 $ 
\end{theorem}

\begin{proof} 
    $\Leftarrow$
    Without loss of generality take, $x = 0$
    Then we get,  \[
        0y
    .\] 
    We can write this as, \[
        (0 + 0)y = 0y + 0y
    .\] 
    So, \[
    0y = 0y + 0y
    .\] 
    Or, m

    $\Rightarrow$

    Assume the contrary that, $x \neq 0 \text{ and } y \neq 0$ 
    We have, $xy = 0$.
    Without loss of generality we take the multiplicative inverse of  $x$ so,
     \[
    \frac{xy}{x} = \frac{0}{x}
    .\] 
    We showed that $0(k) = 0$ so  $y = 0$

    Which contradicts our assumption, hence our asusmptoin must be wrong and  $x = 0 \text{ or } y = 0$
    
\end{proof}
\begin{theorem}
    $(-)x = -x$
\end{theorem}

\begin{proof}
    We start with $(-1)x$ and add $x$ to both sides so,  \[
        (-1)x + x = x (1 - 1) = 0x = 0
    .\] 
    So we showed that $(-1)x$ is the additive identity of $x$. 

    We know that the additive identity is unique for any  $x$

    Therefore,  $(-1)x = -x$
\end{proof}

\begin{theorem}
    $\forall x < y, z < 0$  \[
    xz > yz
    .\] 
\end{theorem}
\begin{proof}

    If $z < 0$ then that means  $z = -k$ for some  $k > 0$.

    We can write $x < y $ as  $x - y < 0$

    Now if we multiply both sides be $k$ we get, 
    $$ k(x - y) < 0 $$ 

    Now if $k (x - y) = z'$  we can say that $z' < 0 \implies -z' > 0$

    Or that  
    $$ (-1)k(x-y) > 0$$ 
    $$z(x-y) > 0$$ 
    $$ xz > yz $$ 

\end{proof}

\begin{theorem}
    $\forall x \in \R$ if $x \neq 0$ then  $x^2> 0$
\end{theorem}

\begin{theorem}
    $x^2 = - (-x^2)$

    Case 1, $x > 0$: 
    $$x > 0$$
    $$x\times x > x$$
    $$x\times x > 0x$$
    $$ x^2 > 0$$
    
    Case 2, $x < 0$:
    
    $$ x < 0 $$ 
    
    Then the additive inverse $(-x) > 0$
     
    $$ (-x)(-x) > (-x)0 $$ 
    $$ (-)(-1)x^2 > 0 $$ 
    $-(-1) = 1$ as  $1$ is the additive inverse of $-1$
    $$ x^2 > 0 $$ 

\end{theorem}

\begin{eg}
    $\forall a,b > 0$  \[
        \frac{a + b}{2} \geq \sqrt{ab}
\end{eg}

\begin{proof}
    \[
        0 \leq (\sqrt{a} - \sqrt{b})^2 = a - 2\sqrt{ab} + b
    .\]      
    
    $$2\sqrt{ab} \le a + b$$
    $$\sqrt{ab} \le \frac{a + b}{2}$$
\end{proof}

\begin{eg}
    $x^2 - x + 1$
\end{eg}



\begin{theorem}
    $\forall x,y \in \R$ we have,  \[
        |x| \geq x \text{ and } |x + y| \leq |x| + |y|
    .\] 

\end{theorem}

\begin{proof}
    We use proof by cases.
    
\end{proof}


\subsection*{Proof related to Sets}
\begin{theorem}
    \[
    A \cup B \backslash (A \cap B) = (A \backslash B) \cup (B \backslash A)
    .\] 

\end{theorem}

\begin{proof}
    We need to show that, \[
 A \cup B \backslash (A \cap B) \subseteq  (A \backslash B) \cup (B \backslash A)
    .\] 
    and,
  \[
  (A \backslash B) \cup (B \backslash A) \subseteq A \cup B \backslash (A \cap B) 
  .\] 
\end{proof}



\begin{theorem}
    $A \subseteq B \iff A \cup B = B$
\end{theorem}

 \begin{proof}
    $\Rightarrow$   
    Take $\forall x \in A \cup B$, so either
    
    Case 1, $x \in A$:

    We know that by deifnition if, $A \subseteq B$ then for  $x \in A, x \in B$ so  $x \in B$
    
    Case 2, $x \in B$:
    If $x \in B$ then we don't need to go further.


    So we get $\forall x \in A \cup B$,  $x \in B$

    $\impliedby$

    $\forall x \in A \Rightarrow x \in A \cup B = B$

    So,  $x \in B$ which means that, $A \subseteq B$
    
\end{proof}



