\section{19. Derivatives}
\begin{theorem}
   If a function $f(z)$ is continuous and non-zero at a point $z_0$ then, there exists a neighborhood where, $f(z) \neq 0$ throughout.
\end{theorem}
\begin{proof}
   
   We know that $f(z)$ is continuous which means that, $\foall \epsilon > 0, \exists \delta$ such that,  \[
      |f(z) - f(z_0)| < \epsilon, \text{ when } 0 < |z - z_0| < \delta
   .\] 

   But if we take, $\epsilon = \frac{f(z_0)}{2}$ then we have, \[
   |f(z) - f(z_0)| < \frac{|f(z_0)|}{2}
   .\] 
   However, if $f(z) = 0$ for this neighborhood then we have,  \[
   |f(z_0)|  < \frac{|f(z_0)|}{2}
   .\] 
   which is a contradiction.



\end{proof}

\begin{theorem}
   $f$ is continuous on $R$ which is closed and bounded, $\exists M > 0$, real $|f(z)| \leq M, \forall z \in R$  equality holds for at least one  $z$.
\end{theorem}


\begin{definition}[Derivative]
   $f$ is differntiable at $z_0$ when $f'(z_0)$ exists where, 
   $$f'(z_0) = \lim_{z \to z_0} \frac{f(z) - f(z_0)}{z-z_0}$$
\end{definition}
\begin{remark}
   Can also solve, \[
   \lim_{z_0 \to 0} \frac{f(z + z_0) - f(z)}{z_0}$$
   .\] 
\end{remark}

\begin{eg}
   Find derivative of, $f(z) = \frac{1}{z}$

   $$\lim_{z_0 \to 0} (\frac{1}{z + z_0} - \frac{1}{z}) \frac{1}{z_0}$$
   $$\lim_{z_0 \to 0} \frac{z - z - z_0}{z(z + z_0)} \frac{1}{z_0}$$
   $$\lim_{z_0 \to 0} \frac{-1}{z(z + z_0)}$$
   $$= \frac{-1}{z^2}$$
\end{eg}
\begin{eg}
   $f(z) = \bar z$

   $$\lim_{z_0 \to 0} \frac{\bar{z + z_0} - \bar z}{z_0}$$

   Go from $x$ and  $y$ axis.

   From $x$,  \[
   \lim_{x_0 \to 0} \frac{\bar z + x_0 - \bar z}{x_0}
   =1
   .\] 
   Similarly if we go from $y$ we get  $-1$, so the derivative doesn't exist.


\end{eg}

If we have a function $f(z) = u(x,y) + iv(x,y)$ then, \[
z_0 = x_0 + iy_0
.\] 
\[
\Delta z = \Delta x + i \Delta y
.\] 

We have to show the following exist, \[
\lim_{\Delta z \to 0} \frac{f(z_0 + \Delta z) - f(z_0)}{\Delta z} .\] 
\[
= \frac{u(x_0 + \Delta x, y_0 + \Delta y) + iv(x_0+\Delta x, y_0 + \Delta y) - (u(x_0,y_0) + iv(x_0,y_0))}{\Delta x + i\Delta y}
.\] 
Horizontally, \Delta y = 0.

So, 
\[\frac{u(x_0 + \Delta x, y_0) - u(x_0,y_0)}{\Delta x} + \frac{i(v(x_0 + \Delta x, y_0) - v(x_0,y_0))}{\Delta x}
.\] 
\[
 = u_x + iv_x
.\] 

Similary, if we go vertically, $\Delta x = 0$ and we get,  \[
= v_y - iu_y
.\] 


\begin{theorem}
   If, $f(z) = u + iv, f'(z)$ exists at,  $z_0 = x_0 + iy_0$. Then, $u_x, u_y, v_x, v_y$ eixsts at  $(x_0, y_0)$ and must satisify the Cauchy-Reimann equation.
   \[
      f'(z_0) = u_x + iv_x \text { at } (x_0,y_0)
   .\] 
\end{theorem}

\begin{theorem}
   $f(z) = u(x,y) + iv(x,y)$ defined throughout the $\epsilon$-neighborhood of $z_0 = x_0 + iy_0$, 

   (a) $u_x,u_y,v_x,v_y$ exists everywhere in the neighborhood

   (b)  $u_x, u_y, v_x, v_y$ continuous at  $(x_0,y_0)$ and satisfy the Cauchy-Remainn equations $$u_x = v_y, u_y = -v_x \text{ at }  (x_0,y_0)$$

   Then $f'(z_0)$  exists and, \[
      f'(z_0) = u_x + iv_x \text{ at } (x_0,y_0)
   .\]
\end{theorem}
\begin{proof}
   We need to show,
   \[
   \lim_{\Delta z \to 0} \frac{f(z_0 + \Delta z) - f(z_0)}{\Delta z}
   .\] 

   \[
   = \lim_{\Delta z \to 0} \frac{u(x_0+ \Delta x, y_0 + \Delta y) + iv(x_0+ \Delta x, y_0 + \Delta y) - (u(x_0,y_0) + iv(x_0,y_0))}{\Delta z}
.\]
Using taylor expansion we know, \[
f(x + \Delta x) = f(x) + \Delta xf'(x) + \frac{(\Delta x)^2}{2}f''(x)
.\] 
\[
   u(x_0+\Delta x, y_0 + \Delta y) - u(x_0,y_0)  = 
\]   
\[
   = u(x_0,y_0) + \Delta x u_x(x_0,y_0) + \frac{(\Delta x)^2}{2} u_{xx}(x_0,y_0) + \Delta y u_y(x_0, y_0) + \frac{(\Delta y)^2}{2}u_{yy} (x_0, y_0) 
.\] 


We can write the limit as, \[
   \frac{u_x(x_0,y_0)\Delta x + u_y (x_0,y_0)\Delta y +  \epsilon_1(\Delta x^2) + \epsilon_2(\Delta y^2)}{\Delta z} + 
\] 
\[
   i\frac{v_x(x_0,y_0)\Delta x + v_y(x_0,y_0)\Delta y + \epsilon_3(\Delta x) + \epsilon_4(\Delta y)}{\Delta z}
.\] 


We know $u_x(x_0,y_0) = v_y(x_0,y_0)$ and $u_y(x_0,y_0) = - v_x(x_0,y_0)$, so,
\[
   \frac{u_x(x_0,y_0)\Delta x + -v_x (x_0,y_0)\Delta y +  \epsilon_1(\Delta x^2) + \epsilon_2(\Delta y^2)}{\Delta z} + 
\] 
\[
   i\frac{v_x(x_0,y_0)\Delta x + u_x(x_0,y_0)\Delta y + \epsilon_3(\Delta x) + \epsilon_4(\Delta y)}{\Delta z}
.\] 

\[
= \frac{u_x(x_0,y_0)(\Delta x + i \Delta y) + u_y(x_0,y_0)(\Delta y - i\Delta x) + \epsilon_4}{\Delta z}
.\] 


and $\Delta z = \Delta x + i \Delta y$

\[
= \frac{u_x(x_0,y_0)(\Delta x + i \Delta y) + u_y(x_0,y_0)(\Delta y - i\Delta x) + \epsilon_4}{\Delta x + i \Delta y}
.\] 


\end{proof}

