\section{Branch Cuts}
\begin{eg}
   $z = 3e^{i\theta}, (0 \le \theta \le \pi)$
\end{eg}



\begin{lemma}
   If $w(t)$ is piecewise cont. then, 
   $$ \bigg | \int_a^b w(t) dt \bigg| \le \int_a^b |w(t)| dt$$       
\end{lemma}
\begin{proof}
   Let, 
   $$\int_a^b w(t) dt = re^{i\theta}$$

   $r = \int_a^b e^{-i\theta}w(t)dt$. Both sides of this equations are real.

   $$r = \int_a^b Re[e^{i\theta}w(t)]dt$$ 

   But, 
$$Re[e^{i\theta}w(t)] \le |e^{-i\theta}w(t)| = |e^{-i\theta}||w(t)| \le |w(t)|$$ 

So, 
$$ r \le \int_a^b |w(t)| dt $$ 
Or, 
$$ \bigg|\int_a^b w(t) dt \bigg| \le \int_a^b |w(t)|dt $$ 
\end{proof}

\begin{theorem}
   $C$ has a length $L$ and $f(z)$ is piecewise cont. on $C$ and let $|f(z)| \le M$ then, 
   $$ \bigg |\int_C f(z) dz \bigg | \le  ML  $$ 
\end{theorem}
\begin{proof}
   $\int_C f(z) dz = \int_a^b f(z(t)) z'(t) dt$. So we have, 
   $$ \bigg | \int_C f(z)dz \bigg | \le \int_a^b |f(z(t))z'(t)|dt \le \int_a^b |Mz'(t)|dt  = ML$$ 
\end{proof}


\begin{theorem}
   $f(z)$ is cont. over $D$ then, 

   (a). $f(z)$ has antiderivative $F(z)$ throughout D

   (b). $\int_{z_1}^{z_2} f(z) dz = F(z_2) - F(z_1)$

   The antiderivative is independent to the path.


   (c). $\int_C f(z)$ where $c$ is a closed contour entirely in $D$
\end{theorem}

\begin{proof}
   1. (a) $\implies$ (b). We have, $c: z= z(t), z_1 = z(a), z_2 = z(b)$
   $$\frac{d}{dt} [F[z(t)]] = F'[z(t)] z'(t) = f(z) z'(t)$$

   So taking, 
   $$ \int_C f(z) dz = \int_a^b f[z(t)]z'(t) dt = F[z(t)]$$ 
   
   $$ = F[z(t)]_a^{b} = F(z_2) - F(z_1)  $$ 

   2. (b) $\implies$ (c)

   $$\int_{C_1} f(z) dz = F(z_2) - F(z_1)$$
   $$\int_{C_2} f(z) dz = F(z_2) - F(z_1)$$
   So, 
   $$\int_{C_1} f(z) dz = F(z_2) - F(z_1) = \int_{C_2} f(z) dz = F(z_2) - F(z_1)$$
   $$\int_{C_1} f(z) dz = F(z_2) - F(z_1) - \int_{C_2} f(z) dz = F(z_2) - F(z_1) = 0$$

   $C = C_1 - C_2:$ a closed contour in $D$ 

   
   $$ \int_C f(z) dz = 0 $$ 


   3. (c) $\implies$ (a)

   We define  $$F(z) = \int_{z_1}^{z_2} f(s) ds$$

   
   $$ \lim_{\Delta z \to 0}  \frac{F(z + \Delta z) - F(z)}{\Delta z} = \lim_{\Delta z \to 0} \frac{1}{\Delta z}\bigg[ \int_{z_0}^{z + \Delta z} f(s) ds - \int_{z_0}^{z} f(z) ds \bigg ]$$ 
   
   $$ = \lim_{\Delta z \to 0} \frac{1}{\Delta z}\int_z^{z+\Delta z} f(s) ds $$ 

\begin{remark}
   $$\int_z^{z + \Delta z} ds = s]_z^{z + \Delta z} = \Delta z$$
\end{remark}
\begin{remark}
   $$ f(z) = \frac{1}{\Delta z} \int_z^{z + \Delta z} f(z) ds$$ 
\end{remark}



$$ \frac{F(z + \Delta z) - F(z)}{\Delta z} - f(z) = \frac{1}{\Delta z} \int_z^{z + \Delta z} [f(s) - f(z)] ds $$ 

By cont. of $f(z), \forall \epsilon, \exists \delta$,  
$$ |f(s) - f(z)| < \epsilon \text{ whenever } |s - z| < \delta $$


\end{proof}




