\documentclass[a4paper]{report}
\input{preamble.tex}
\title{MATH 4320 HW03}
\author{Aamod Varma}
\begin{document}
\maketitle


\subsection*{Problem 3}
(a). $lim_{z \rightarrow z_o} \frac{1}{z^n}(z_0 \neq 0)$

We know, $$lim_{z \rightarrow z_o} \frac{1}{z^n} = \frac{lim_{z \rightarrow z_0}1} {lim_{z \rightarrow z_0}{z^n}} = \frac{1}{z_0^n}$$

(b). $lim_{z \rightarrow i} \frac{iz^3 - 1}{z + i}$


We know, $$lim_{z \rightarrow i} \frac{iz^3 - 1}{z + i} = \frac{lim_{z \rightarrow z_0}iz^3 - 1} {lim_{z \rightarrow z_0}{z + i}} = \frac{i^4 - 1}{2i} = \frac{0}{2i} = 0$$


(c). $lim_{z \rightarrow z_0} \frac{P(z)}{Q(z)}$

We know, $$lim_{z \rightarrow z_0} \frac{P(z)}{Q(z)} = \frac{lim_{z \rightarrow z_0}P(z)} {lim_{z \rightarrow z_0}{Q(z)}} = \frac{P(z_0)}{Q(z_0)}$$




\subsection*{Problem 7}
Using the definition of limits we know that, $\forall \epsilon > 0, \exists \delta$ such that. \[
    |f(z) - w_0| < \epsilon \text{ whenever } 0 < z - z_0 < \delta
.\] 
We know from the triangle inequality that, \[
|a - b| \ge ||a| - |b||
.\] 
Using this we can say, \[
||f(z)| - |w_0|| \le |f(z) - w_0|
.\] 

So we have, \[
||f(z)| - |w_0|| < \epsilon
.\] 

Now using the definition of limits once again, we get $\forall \epsilon > 0, \exists \delta$ the same as before, such that  \[
    ||f(z)| - |w_0|| < \epsilon \text{ whenever } 0 < |z - z_0| < \delta
.\] 
This shows that we can write, \[
\lim_{z \to z_0} |f(z)| = |w_0|
.\] 

\subsection*{Problem 10}
(a). $\lim_{z \to \infty} \frac{4z^2}{(z-1)^2} = 4$ 

We know that, \[
\lim_{z \to 0} f\bigg (\frac{1}{z}\bigg ) = w_0
.\] 
then, \[
\lim_{z \to \infty} f(z) = w_0
.\] 

So we can say, \[
    \lim_{z \to \infty} \frac{4z^2}{(z-1)^2} = \lim_{z \to 0} \frac{\frac{4}{z^2}}{(\frac{1}{z} - 1)^2}
.\]
\[
    = \lim_{z \to 0} \frac{4}{(1 - z)^2}
.\] 
\[
    = \frac{4}{1-0} = 4
.\] 

(b). $\lim_{z \to 1} \frac{1}{(z-1)^3} = \infty$

Using theorem we know that, \[
    \lim_{z \to z_0} f(z) = \infty \text{ if } \lim_{z \to z_0} \frac{1}{f(z)} = 0
.\] 
\[
    \lim_{z \to 1} \frac{(z-1)^3}{1} = \frac{(1-1)^3}{1} = 0
.\] 
So using the theorem we get, \[
 \lim_{z \to 1} \frac{1}{(z-1)^3} = \infty
.\] 

(c). $\lim_{z \to \infty} \frac{z^2 + 1}{z-1} = \infty$
Using theorem we know that, \[
    \lim_{z \to \infty} f(z) = \infty \text{ if } \lim_{z \to 0} \frac{1}{f(\frac{1}{z})} = 0
.\] 

Using this, \[
    \lim_{z \to 0} \frac{\frac{1}{z} - 1}{\frac{1}{z^2} + 1} = \frac{1 - 1}{1 + 1} = 0
.\]         

So, \[
 \lim_{z \to \infty} \frac{z^2 + 1}{z-1} = \infty
.\] 
\end{document}
